src/TwoExecExample.v
@@ -1,0 +1,233 @@
+(** this axioms may simplify tree equivalence after execution proofs *)
+Axiom one_tag_per_user:
+  forall pr t t',
+    t <> Public ->
+    t' <> Public ->
+    can_access pr t ->
+    can_access pr t' ->
+    t = t'.
+
+Axiom one_user_per_tag:
+  forall pr pr' t,
+    t <> Public ->
+    can_access pr t ->
+    can_access pr' t ->
+    pr = pr'.
+
+
+Definition sys_rep Fr Fm Ftop fsxp ds sm tree ilist frees mscs bm hm:=
+  (Fr * [[ sync_invariant Fr ]] *
+   LOG.rep (FSXPLog fsxp) (SB.rep fsxp) (LOG.NoTxn ds) (MSLL mscs) sm bm hm *
+   [[[ ds!! ::: (Fm * rep fsxp Ftop tree ilist frees mscs sm)]]])%pred.
+
+
+
+
+
+
+
+
+
+
+
+
+
+
+
+Lemma two_exec_return_indistinguishable:
+  forall T (p: fprog T) pathname f pr off vs inum Fd tag
+    Fr1 Fm1 Ftop1 ds1 sm1 tree1 mscs1 mscs1' fsxp1 ilist1 frees1 d1 bm1 hm1 d1' bm1' hm1' tr1 tr1'
+    Fr2 Fm2 Ftop2 ds2 sm2 tree2 mscs2 mscs2' fsxp2 ilist2 frees2 d2 bm2 hm2 d2' bm2' hm2' tr2 tr2'
+    (r1 r2: T),
+    
+  fexec pr tr1 d1 bm1 hm1 mscs1 p (RFinished d1' bm1' hm1' r1) mscs1' tr1' ->
+  fexec pr tr2 d2 bm2 hm2 mscs2 p (RFinished d2' bm2' hm2' r2) mscs2' tr2' ->
+
+  
+  (sys_rep Fr1 Fm1 Ftop1 fsxp1 ds1 sm1 tree1 ilist1 frees1 mscs1 bm1 hm1)%pred d1 ->
+  (sys_rep Fr2 Fm2 Ftop2 fsxp2 ds2 sm2 tree2 ilist2 frees2 mscs2 bm2 hm2)%pred d2 ->
+
+  (** this represents the residual part of the precondition.
+  e.g. a file existing and file having a block in the given offset etc. *)
+  satisfies_precondition tree1 p ->
+  satisfies precondition tree2 p ->
+  
+  can_access pr tag ->
+  equivalent_for tag tree1 tree2 ->
+  r1 = r2.
+
+
+
+
+
+
+
+
+
+  
+
+  
+
+
+  
+
+(** This is an alternative, stronger lemma which requires 
+    proving an existence of a successful execution from equivalent tree. 
+    I am not sure this version is provable in our framnework. **)
+Lemma two_exec_return_indistinguishable_alternative:
+  forall T (p: fprog T) pathname f pr off vs inum Fd tag
+    Fr1 Fm1 Ftop1 ds1 sm1 tree1 mscs1 fsxp1 ilist1 frees1 d1 bm1 hm1 tr1 d1' bm1' hm1' mscs1' tr1'
+    Fr2 Fm2 Ftop2 ds2 sm2 tree2 mscs2 fsxp2 ilist2 frees2 d2 bm2 hm2 tr2
+    (r1 r2: T),
+    
+  fexec pr tr1 d1 bm1 hm1 mscs1 p (RFinished d1' bm1' hm1' r1) mscs1' tr1' ->
+  
+  (sys_rep Fr1 Fm1 Ftop1 fsxp1 ds1 sm1 tree1 ilist1 frees1 mscs1 bm1 hm1)%pred d1 ->
+  (sys_rep Fr2 Fm2 Ftop2 fsxp2 ds2 sm2 tree2 ilist2 frees2 mscs2 bm2 hm2)%pred d2 ->
+
+  (** this represents the residual part of the precondition.
+  e.g. a file existing and file having a block in the given offset etc. *)
+  satisfies_precondition tree1 p ->
+  satisfies precondition tree2 p ->
+  
+  can_access pr tag ->
+  equivalent_for tag tree1 tree2 ->
+  
+  exists d2' bm2' hm2' r2 mscs2' tr2',
+    fexec pr tr2 d2 bm2 hm2 mscs2 p (RFinished d2' bm2' hm2' r2) mscs2' tr2' /\
+    r1 = r2.
+
+
+
+
+
+
+
+
+
+
+
+
+
+
+
+
+
+  
+(** This lemma proves that -combined with two_exec_return_indistinguishable- 
+   interleaving syscalls from different users will preserve isolation.
+   it inforamlly states the parts that user pr can't reach will stay equivalent 
+   after series of syscalls from that user. **)
+  Lemma two_exec_no_effect_on_others:
+  forall T (p: fprog T) pathname f pr off vs inum Fd tag tag'
+    Fr1 Fm1 Ftop1 ds1 sm1 tree1 mscs1 mscs1' fsxp1 ilist1 frees1 d1 bm1 hm1 d1' bm1' hm1' tr1 tr1'
+    Fr2 Fm2 Ftop2 ds2 sm2 tree2 mscs2 mscs2' fsxp2 ilist2 frees2 d2 bm2 hm2 d2' bm2' hm2' tr2 tr2'
+    (r1 r2: T),
+    
+  fexec pr tr1 d1 bm1 hm1 mscs1 p (RFinished d1' bm1' hm1' r1) mscs1' tr1' ->
+  fexec pr tr2 d2 bm2 hm2 mscs2 p (RFinished d2' bm2' hm2' r2) mscs2' tr2' ->
+
+  
+  (sys_rep Fr1 Fm1 Ftop1 fsxp1 ds1 sm1 tree1 ilist1 frees1 mscs1 bm1 hm1)%pred d1 ->
+  (sys_rep Fr2 Fm2 Ftop2 fsxp2 ds2 sm2 tree2 ilist2 frees2 mscs2 bm2 hm2)%pred d2 ->
+
+  (** this represents the residual part of the precondition.
+  e.g. a file existing and file having a block in the given offset etc. *)
+  satisfies_precondition tree1 p ->
+  satisfies precondition tree2 p ->
+  
+  can_access pr tag ->
+  tag <> tag' ->
+  equivalent_for tag' tree1 tree2 ->
+
+  exists ds1' sm1' tree1' ilist1' frees1' ds2' sm2' tree2' ilist2' frees2',
+      (sys_rep Fr1 Fm1 Ftop1 fsxp1 ds1' sm1' tree1' ilist1' frees1' mscs1' bm1' hm1')%pred d1' /\
+      (sys_rep Fr2 Fm2 Ftop2 fsxp2 ds2' sm2' tree2' ilist2' frees2' mscs2' bm2' hm2')%pred d2' /\
+      equivalent_for tag' tree1' tree2'.
+
+
+
+
+
+
+
+
+
+
+
+
+
+
+
+
+
+
+
+
+
+
+
+
+
+
+
+
+
+    
+(** CRASHES **)
+
+
+(** One shortcoming of the below lemma is that 
+    it starts execution from a synced disc. 
+    This requirement is imposed by the second part of the conclusion.
+    if we would allow from some arbitrary disk, 
+    then it could be recovered to a state 
+    that is even before where p starts to execute.
+    If that is the case, I don't know how to prove 
+    the property second part wants to prove. **)
+Lemma two_exec_recover_equivalent:
+  forall T (p: fprog T) pathname f pr off vs inum Fd tag
+    Fr1 Fm1 Ftop1 ds1 sm1 tree1 mscs1 mscs1' fsxp1 ilist1 frees1 d1 bm1 hm1 d1' bm1' hm1' tr1 tr1'
+    Fr2 Fm2 Ftop2 ds2 sm2 tree2 mscs2 mscs2' fsxp2 ilist2 frees2 d2 bm2 hm2 d2' bm2' hm2' tr2 tr2'
+    (r1 r2: T),
+    
+  fexec pr tr1 d1 bm1 hm1 mscs1 p (RRecovered d1' bm1' hm1' r1) mscs1' tr1' ->
+  fexec pr tr2 d2 bm2 hm2 mscs2 p (RRecovered d2' bm2' hm2' r2) mscs2' tr2' ->
+  
+  
+  (sys_rep Fr1 Fm1 Ftop1 fsxp1 (ds1, []) sm1 tree1 ilist1 frees1 mscs1 bm1 hm1)%pred d1 ->
+  (sys_rep Fr2 Fm2 Ftop2 fsxp2 (ds2, []) sm2 tree2 ilist2 frees2 mscs2 bm2 hm2)%pred d2 ->
+
+  (** this represents the residual part of the precondition.
+  e.g. a file existing and file having a block in the given offset etc. *)
+  satisfies_precondition tree1 p ->
+  satisfies precondition tree2 p ->
+  
+  can_access pr tag ->
+  equivalent_for tag tree1 tree2 ->
+
+  exists Fr1' Fm1' Ftop1' fsxp1' ds1' sm1' tree1' ilist1' frees1'
+     Fr2' Fm2' Ftop2' fsxp2' ds2' sm2' tree2' ilist2' frees2',
+
+    (sys_rep Fr1 Fm1 Ftop1 fsxp1 (ds1', []) sm1'
+             tree1' ilist1' frees1' mscs1' bm1' hm1')%pred d1' /\
+    (sys_rep Fr2 Fm2 Ftop2 fsxp2 (ds2', []) sm2'
+             tree2' ilist2' frees2' mscs2' bm2' hm2')%pred d2' /\
+    equivalent_for tag tree1' tree2' /\
+
+  (** this part says that the disks we recovered are reachable by 
+      executing only a prefix of the program p. This has an implication that 
+      we didn't recover a data to a wrong owner **)
+  exists n,
+  (exists d1'' bm1'' hm1'' r1' mscs1'' tr1'' ds1'' sm1'' ilist1'' frees1'',
+     fexec pr tr1 d1 bm1 hm1 mscs1 (firstn_steps n p)
+           (RFinished d1'' bm1'' hm1'' r1') mscs1'' tr1'' /\
+     (sys_rep Fr1 Fm1 Ftop1 fsxp1 ds1'' sm1''
+              tree1' ilist1'' frees1'' mscs1'' bm1'' hm1'')%pred d1'' /\
+     ds1''!! = ds1') /\
+  (exists d2'' bm2'' hm2'' r2' mscs2'' tr2'' ds2'' sm2'' ilist2'' frees2'',
+     fexec pr tr2 d2 bm2 hm2 mscs2 (firstn_steps n p)
+           (RFinished d2'' bm2'' hm2'' r2') mscs2'' tr2'' /\
+     (sys_rep Fr2 Fm2 Ftop2 fsxp2 ds2'' sm2''
+              tree2' ilist2'' frees2'' mscs2'' bm2'' hm2'')%pred d2'' /\
+      ds2''!! = ds2!).
